verified/smcapi.s.dfy
@@ -428,7 +428,8 @@ predicate smchandlerInvariant(s:state, s':state, entry:bool)
         else
             InsecureMemInvariant(s, s')
             && (forall m :: s.regs[LR(m)] == s'.regs[LR(m)])
-            && (forall m | m != User :: s.sregs[spsr(m)] == s.sregs[spsr(m)]))
+            && (forall m | m != User :: s.sregs[spsr(m)] == s'.sregs[spsr(m)]))
+            && s.sregs[cpsr] == s'.sregs[cpsr]
 }
 
 predicate smchandler(s: state, pageDbIn: PageDb, s':state, pageDbOut: PageDb)
